lambda2Gmu/DefinitionsTests.v
@@ -14,7 +14,7 @@ Lemma open_ee_test : open_ee (trm_abs (typ_bvar 0) (trm_bvar 1)) (trm_unit) = tr
   cbv. auto.
 Qed.
 
-Lemma open_typlist_test : open_typlist_rec 0 (typ_unit) [typ_bvar 0; typ_tuple (typ_bvar 0) (typ_bvar 1)] = [typ_unit; typ_tuple (typ_unit) (typ_bvar 0)].
+Lemma open_typlist_test : open_typlist_rec 0 (typ_unit) [typ_bvar 0; typ_tuple (typ_bvar 0) (typ_bvar 1)]* = [typ_unit; typ_tuple (typ_unit) (typ_bvar 0)]*.
   cbv; repeat case_if. auto.
 Qed.
 
@@ -24,11 +24,11 @@ Hypothesis T : var.
 (* Lemma open_tt_many_test : open_tt_many [typ_unit; typ_fvar T] (typ_tuple (typ_bvar 0) (typ_bvar 1)) = typ_tuple typ_unit (typ_fvar T). *)
 (*   cbv. auto. *)
 (* Qed. *)
-Lemma open_tt_many_test : open_tt_many [typ_fvar T; typ_unit] (typ_tuple (typ_bvar 0) (typ_bvar 1)) = typ_tuple typ_unit (typ_fvar T).
+Lemma open_tt_many_test : open_tt_many [typ_fvar T; typ_unit]* (typ_tuple (typ_bvar 0) (typ_bvar 1)) = typ_tuple typ_unit (typ_fvar T).
   cbv. auto.
 Qed.
 
-Lemma open_te_many_test : open_te_many [typ_fvar T; typ_unit] (trm_abs (typ_tuple (typ_bvar 0) (typ_bvar 1)) (trm_bvar 0)) = (trm_abs (typ_tuple typ_unit (typ_fvar T)) (trm_bvar 0)).
+Lemma open_te_many_test : open_te_many [typ_fvar T; typ_unit]* (trm_abs (typ_tuple (typ_bvar 0) (typ_bvar 1)) (trm_bvar 0)) = (trm_abs (typ_tuple typ_unit (typ_fvar T)) (trm_bvar 0)).
   cbv. auto.
 Qed.
 
